try to use known() trick to limit reachability axiom instantiations

misc/queue.bpl
@@ -332,10 +332,12 @@ procedure {:yields} {:layer 1} {:refines "offer_spec"}
   var t, tn: Loc;
   var b: bool;
   var x: Loc; var {:linear "FP"} x_FP: [Loc]bool;
-  yield; assert {:layer 1} Inv(heap, head, tail, queue_FP, lin, vis, called, returned);
+  yield; assert {:layer 1} Inv(heap, head, tail, queue_FP, lin, vis, called, returned);  assert {:layer 1} knownF(next(heap));
 
   call x, x_FP := alloc();
 
+  assert {:layer 1} knownF(next(heap)) && known(head) && known(tail) && known(x) && known(null);
+  assert {:layer 1} BetweenSet(next(heap), head, null) == queue_FP;
   yield; assert {:layer 1} Inv(heap, head, tail, queue_FP, lin, vis, called, returned);
   assert {:layer 1} !Between(next(heap), head, x, null);
   assert {:layer 1} dom(heap)[x];
@@ -389,6 +391,13 @@ procedure {:yields} {:layer 1} {:refines "offer_spec"}
 
 // ---------- Reachability, between, and associated theories
 
+// Predicates used to control the triggers on the below axioms
+function known(x: Loc) : bool;
+function knownF(f: [Loc]Loc) : bool;
+axiom(forall x: Loc :: {known(x)} known(x));
+axiom(forall f: [Loc]Loc :: {knownF(f)} knownF(f));
+
+ 
 function Equal([Loc]bool, [Loc]bool) returns (bool);
 function Subset([Loc]bool, [Loc]bool) returns (bool);
 
@@ -422,9 +431,9 @@ function BetweenSet(f: [Loc]Loc, x: Loc, z: Loc) returns ([Loc]bool);
 ////////////////////////////////////////////////////
 // axioms relating Between and BetweenSet
 ////////////////////////////////////////////////////
-axiom(forall f: [Loc]Loc, x: Loc, y: Loc, z: Loc :: {BetweenSet(f, x, z)[y]} BetweenSet(f, x, z)[y] <==> Between(f, x, y, z));
-axiom(forall f: [Loc]Loc, x: Loc, y: Loc, z: Loc :: {Between(f, x, y, z), BetweenSet(f, x, z)} Between(f, x, y, z) ==> BetweenSet(f, x, z)[y]);
-axiom(forall f: [Loc]Loc, x: Loc, z: Loc :: {BetweenSet(f, x, z)} Between(f, x, x, x));
+axiom(forall f: [Loc]Loc, x: Loc, y: Loc, z: Loc :: {knownF(f), known(x), known(y), known(z)} BetweenSet(f, x, z)[y] <==> Between(f, x, y, z));
+axiom(forall f: [Loc]Loc, x: Loc, y: Loc, z: Loc :: {knownF(f), known(x), known(y), known(z)} Between(f, x, y, z) ==> BetweenSet(f, x, z)[y]);
+axiom(forall f: [Loc]Loc, x: Loc :: {knownF(f), known(x)} Between(f, x, x, x));
 axiom(forall f: [Loc]Loc, x: Loc, z: Loc :: {BetweenSet(f, x, z)} Between(f, z, z, z));
 
 
@@ -436,43 +445,43 @@ axiom(forall f: [Loc]Loc, x: Loc, z: Loc :: {BetweenSet(f, x, z)} Between(f, z, 
 axiom(forall f: [Loc]Loc, x: Loc :: Between(f, x, x, x));
 
 // step
-axiom(forall f: [Loc]Loc, x: Loc, y: Loc, z: Loc, w:Loc :: {Between(f, y, z, w), f[x]} Between(f, x, f[x], f[x]));
+axiom(forall f: [Loc]Loc, x: Loc :: {f[x]} Between(f, x, f[x], f[x]));
 
 // reach
-axiom(forall f: [Loc]Loc, x: Loc, y: Loc :: {f[x], Between(f, x, y, y)} Between(f, x, y, y) ==> x == y || Between(f, x, f[x], y));
+axiom(forall f: [Loc]Loc, x: Loc, y: Loc :: {f[x], known(y)} Between(f, x, y, y) ==> x == y || Between(f, x, f[x], y));
 
 // cycle
-axiom(forall f: [Loc]Loc, x: Loc, y:Loc :: {f[x], Between(f, x, y, y)} f[x] == x && Between(f, x, y, y) ==> x == y);
+axiom(forall f: [Loc]Loc, x: Loc, y:Loc :: {f[x], known(y)} f[x] == x && Between(f, x, y, y) ==> x == y);
 
 // sandwich
-axiom(forall f: [Loc]Loc, x: Loc, y: Loc :: {Between(f, x, y, x)} Between(f, x, y, x) ==> x == y);
+axiom(forall f: [Loc]Loc, x: Loc, y: Loc :: {knownF(f), known(x), known(y)} Between(f, x, y, x) ==> x == y);
 
 // order1
-axiom(forall f: [Loc]Loc, x: Loc, y: Loc, z: Loc :: {Between(f, x, y, y), Between(f, x, z, z)} Between(f, x, y, y) && Between(f, x, z, z) ==> Between(f, x, y, z) || Between(f, x, z, y));
+axiom(forall f: [Loc]Loc, x: Loc, y: Loc, z: Loc :: {knownF(f), known(x), known(y), known(z)} Between(f, x, y, y) && Between(f, x, z, z) ==> Between(f, x, y, z) || Between(f, x, z, y));
 
 // order2
-axiom(forall f: [Loc]Loc, x: Loc, y: Loc, z: Loc :: {Between(f, x, y, z)} Between(f, x, y, z) ==> Between(f, x, y, y) && Between(f, y, z, z));
+axiom(forall f: [Loc]Loc, x: Loc, y: Loc, z: Loc :: {knownF(f), known(x), known(y), known(z)} Between(f, x, y, z) ==> Between(f, x, y, y) && Between(f, y, z, z));
 
 // transitive1
-axiom(forall f: [Loc]Loc, x: Loc, y: Loc, z: Loc :: {Between(f, x, y, y), Between(f, y, z, z)} Between(f, x, y, y) && Between(f, y, z, z) ==> Between(f, x, z, z));
+axiom(forall f: [Loc]Loc, x: Loc, y: Loc, z: Loc :: {knownF(f), known(x), known(y), known(z)} Between(f, x, y, y) && Between(f, y, z, z) ==> Between(f, x, z, z));
 
 // transitive2
-axiom(forall f: [Loc]Loc, x: Loc, y: Loc, z: Loc, w: Loc :: {Between(f, x, y, z), Between(f, y, w, z)} Between(f, x, y, z) && Between(f, y, w, z) ==> Between(f, x, y, w) && Between(f, x, w, z));
+axiom(forall f: [Loc]Loc, x: Loc, y: Loc, z: Loc, w: Loc :: {knownF(f), known(x), known(y), known(z), known(w)} Between(f, x, y, z) && Between(f, y, w, z) ==> Between(f, x, y, w) && Between(f, x, w, z));
 
 // transitive3
-axiom(forall f: [Loc]Loc, x: Loc, y: Loc, z: Loc, w: Loc :: {Between(f, x, y, z), Between(f, x, w, y)} Between(f, x, y, z) && Between(f, x, w, y) ==> Between(f, x, w, z) && Between(f, w, y, z));
+axiom(forall f: [Loc]Loc, x: Loc, y: Loc, z: Loc, w: Loc :: {knownF(f), known(x), known(y), known(z), known(w)} Between(f, x, y, z) && Between(f, x, w, y) ==> Between(f, x, w, z) && Between(f, w, y, z));
 
 // This axiom is required to deal with the incompleteness of the trigger for the reflexive axiom.
 // It cannot be proved using the rest of the axioms.
-axiom(forall f: [Loc]Loc, u:Loc, x: Loc :: {Between(f, u, x, x)} Between(f, u, x, x) ==> Between(f, u, u, x));
+axiom(forall f: [Loc]Loc, u:Loc, x: Loc :: {knownF(f), known(x), known(u)} Between(f, u, x, x) ==> Between(f, u, u, x));
 
 // relation between Avoiding and Between
-axiom(forall f: [Loc]Loc, x: Loc, y: Loc, z: Loc :: {Avoiding(f, x, y, z)} Avoiding(f, x, y, z) <==> (Between(f, x, y, z) || (Between(f, x, y, y) && !Between(f, x, z, z))));
-axiom(forall f: [Loc]Loc, x: Loc, y: Loc, z: Loc :: {Between(f, x, y, z)} Between(f, x, y, z) <==> (Avoiding(f, x, y, z) && Avoiding(f, x, z, z)));
+axiom(forall f: [Loc]Loc, x: Loc, y: Loc, z: Loc :: {knownF(f), known(x), known(y), known(z)} Avoiding(f, x, y, z) <==> (Between(f, x, y, z) || (Between(f, x, y, y) && !Between(f, x, z, z))));
+axiom(forall f: [Loc]Loc, x: Loc, y: Loc, z: Loc :: {knownF(f), known(x), known(y), known(z)} Between(f, x, y, z) <==> (Avoiding(f, x, y, z) && Avoiding(f, x, z, z)));
 
 // update
-axiom(forall f: [Loc]Loc, u: Loc, v: Loc, x: Loc, p: Loc, q: Loc :: {Avoiding(f[p := q], u, v, x)} Avoiding(f[p := q], u, v, x) <==> ((Avoiding(f, u, v, p) && Avoiding(f, u, v, x)) || (Avoiding(f, u, p, x) && p != x && Avoiding(f, q, v, p) && Avoiding(f, q, v, x))));
+axiom(forall f: [Loc]Loc, u: Loc, v: Loc, x: Loc, p: Loc, q: Loc :: {knownF(f), known(x), known(u), known(v), known(p), known(q)} Avoiding(f[p := q], u, v, x) <==> ((Avoiding(f, u, v, p) && Avoiding(f, u, v, x)) || (Avoiding(f, u, p, x) && p != x && Avoiding(f, q, v, p) && Avoiding(f, q, v, x))));
 
-axiom (forall f: [Loc]Loc, p: Loc, q: Loc, u: Loc, w: Loc :: {BetweenSet(f[p := q], u, w)} Avoiding(f, u, w, p) ==> Equal(BetweenSet(f[p := q], u, w), BetweenSet(f, u, w)));
-axiom (forall f: [Loc]Loc, p: Loc, q: Loc, u: Loc, w: Loc :: {BetweenSet(f[p := q], u, w)} p != w && Avoiding(f, u, p, w) && Avoiding(f, q, w, p) ==> Equal(BetweenSet(f[p := q], u, w), Union(BetweenSet(f, u, p), BetweenSet(f, q, w))));
-axiom (forall f: [Loc]Loc, p: Loc, q: Loc, u: Loc, w: Loc :: {BetweenSet(f[p := q], u, w)} Avoiding(f, u, w, p) || (p != w && Avoiding(f, u, p, w) && Avoiding(f, q, w, p)) || Equal(BetweenSet(f[p := q], u, w), Empty()));
+axiom (forall f: [Loc]Loc, p: Loc, q: Loc, u: Loc, w: Loc :: {knownF(f), known(p), known(q), known(u), known(w)} Avoiding(f, u, w, p) ==> Equal(BetweenSet(f[p := q], u, w), BetweenSet(f, u, w)));
+axiom (forall f: [Loc]Loc, p: Loc, q: Loc, u: Loc, w: Loc :: {knownF(f), known(p), known(q), known(u), known(w)} p != w && Avoiding(f, u, p, w) && Avoiding(f, q, w, p) ==> Equal(BetweenSet(f[p := q], u, w), Union(BetweenSet(f, u, p), BetweenSet(f, q, w))));
+axiom (forall f: [Loc]Loc, p: Loc, q: Loc, u: Loc, w: Loc :: {knownF(f), known(p), known(q), known(u), known(w)} Avoiding(f, u, w, p) || (p != w && Avoiding(f, u, p, w) && Avoiding(f, q, w, p)) || Equal(BetweenSet(f[p := q], u, w), Empty()));
